tests/defined/mutual_recursion.c
@@ -1,0 +1,12 @@
+int even(int);
+
+int main() {
+  for (int i = 0; i < 10; i++) printf("even %d = %d\n", i, even(i));
+}
+
+int odd(int x) {
+  if (x == 0) return 0; else return even (x - 1);
+}
+int even(int x) {
+  if (x == 0) return 1; else return odd (x - 1);
+}
